\textbf{(Iterative Solution of Linear Systems.)} Consider the $n \times n$
linear system $Ax=b$ and recall the three iterative techniques we
discussed in class:

\textbf{Gauss-Jacobi:}
\[
x_i^{[k+1]} = \frac{1}{a_{ii}} \left( b_i - \sum_{j=1}^{i-1} a_{ij}
x_j^{[k]} - \sum_{j=i+1}^n a_{ij} x_j^{[k]} \right)
\]

\textbf{Gauss-Seidel:}
\[
x_i^{[k+1]} = \frac{1}{a_{ii}} \left(
b_i - \sum_{j=1}^{i-1} a_{ij} x_j^{[k]} - \sum_{j=i+1}^n a_{ij} x_j^{[k+1]}
\right)
\]

\textbf{Successive Overrelaxation:}
\[
x_i^{[k+1]} =
(1 - w)x_i^{[k]} + \frac{w}{a_{ii}}
\left(
b_i - \sum_{j=1}^{i-1} a_{ij} x_j^{[k]} - \sum_{j=i+1}^n a_{ij} x_j^{[k+1]}
\right)
\]

As we discussed in class, think of $A$ as being split as
\[
A = L + D + U
\]
where $L$ contains the entries of $A$ below the diagonal, $U$ contains
the entries above the diagonal, and $D$ contains the entries on the
diagonal. For example,
\[
A
= \left[\begin{matrix} 1 & 2 \\ 3 & 4 \end{matrix} \right]
= L + D + U
= \left[\begin{matrix} 0 & 0 \\ 3 & 0 \end{matrix} \right]
= \left[\begin{matrix} 1 & 0 \\ 0 & 4 \end{matrix} \right]
= \left[\begin{matrix} 0 & 2 \\ 0 & 0 \end{matrix} \right]
\]

Write the above three iterations as
\[
x^{[k+1]} = T_x^{[k]} + c
\]
and for each of the three methods give $T$ in terms of $L$, $D$, and
$U$, and $c$ in terms of $L$, $D$, $U$ and $b$.

Note: in class we derived the correct expressions for the Gauss-Jacobi
method. There was a mistake in the in-class discussion of the
Gauss-Seidel method, and I left the SOR method as an exercise.

{\color{blue}

\textbf{Gauss-Jacobi:}

\begin{align*}
x_i^{[k+1]} &= \frac{1}{a_{ii}} \left( b_i - \sum_{j=1}^{i-1} a_{ij} x_j^{[k]} - \sum_{j=i+1}^n a_{ij} x_j^{[k]} \right) \\
x^{[k+1] }&= D^{-1} \left( b - L x^{[k]} - U x^{[k]} \right) \\
&= D^{-1} \left( b - \left(L + U\right) x^{[k]} \right) \\
&= -D^{-1} \left( L + U \right) x^{[k]} + D^{-1} b \\
\end{align*}
\begin{align*}
\Rightarrow T &= -D^{-1} \left( L + U \right) \\
c &= D^{-1} b
\end{align*}

\textbf{Gauss-Seidel:}
\begin{align*}
x_i^{[k+1]} &= \frac{1}{a_{ii}} \left(b_i - \sum_{j=1}^{i-1} a_{ij}
x_j^{[k]} - \sum_{j=i+1}^n a_{ij} x_j^{[k+1]} \right) \\
x^{[k+1] }&= D^{-1} \left( b - L x^{[k]} - U x^{[k+1]} \right) \\
x^{[k+1] }&= D^{-1} b - D^{-1} L x^{[k]} - D^{-1} U x^{[k+1]}  \\
(I + D^{-1} U) x^{[k+1]} &= D^{-1} b - D^{-1} L x^{[k]} \\
x^{[k+1]} &= - (I + D^{-1} U)^{-1} D^{-1} L x^{[k]} + (I + D^{-1} U)^{-1} D^{-1} b  \\
\end{align*}
\begin{align*}
\Rightarrow
T &= - (I + D^{-1} U)^{-1} D^{-1} L \\
c &= (I + D^{-1} U)^{-1} D^{-1} b
\end{align*}

\textbf{Successive Overrelaxation:}

\begin{align*}
x_i^{[k+1]} &= (1 - w)x_i^{[k]} + \frac{w}{a_{ii}} \left(b_i
- \sum_{j=1}^{i-1} a_{ij} x_j^{[k]} - \sum_{j=i+1}^n a_{ij}
x_j^{[k+1]} \right) \\
x^{[k+1]} &= \left(1-\omega\right) x^{[k]} + \omega D^{-1} \left( b -
L x^{[k]} - U x^{[k+1]}\right) \\
&= \left( 1 - \omega \right) x^{[k]} + \omega D^{-1} b - \omega
D^{-1} L x^{[k]} - \omega D^{-1} U x^{[k+1]} \\
\left( I + \omega D^{-1} U \right) x^{[k+1]} &= \left( \left( 1
- \omega \right)  - \omega D^{-1} L \right)  x^{[k]} + \omega D^{-1} b \\
x^{[k+1]} &= \left( I + \omega D^{-1} U \right)^{-1} \left( \left( 1
- \omega \right) - \omega D^{-1} L \right) x^{[k]} + \left( I
+ \omega D^{-1} U \right) \omega D^{-1} b
\end{align*}
\begin{align*}
\Rightarrow
T &= \left( I + \omega D^{-1} U \right)^{-1} \left( \left( 1
- \omega \right) - \omega D^{-1} L \right)\\
c &= \left( I + \omega D^{-1} U \right) \omega D^{-1}
\end{align*}

}
