\textbf{A cubically convergent method:} Consider the iteration \[x_{k+1} = g(x_k)\text{    where    }g(x) = x - \frac{f(x)}{f^\prime(x)} - \frac{1}{2} \frac{f^2 (x) f^{\prime \prime} (x)}{\left(f^\prime(x)\right)^3}\]. (We assume $f$ is sufficiently differentiable, and $f^\prime(x) \ne 0$.) Suppose that $g(\alpha) = \alpha$. Show that \[g^\prime(\alpha) = g^{\prime\prime}(\alpha) = 0\]. (Thus the fixed point method will converge of order at least 3 if we start sufficiently close to $\alpha$.)

{\color{blue}

\[
g(x) = x - \frac{f(x)}{f^\prime(x)} - \frac{{f(x)}^2\, f^{\prime \prime}(x)}{2\, { f^\prime(x)}^3}
\]

\[
\begin{aligned}
g^\prime (x)
%&= 1 - \frac{{f^\prime (x)}^2 - f(x)\, f^{\prime \prime}(x)}{f^\prime(x)^2} - \frac{{f^\prime(x)}^3\, \left({f(x)}^2\, f^{(3)}(x) + f(x)\, f^{\prime \prime}(x)\, f^\prime(x)\, 2\right) - 3\, {f(x)}^2\, {f^\prime(x)}^2\, { f^{\prime \prime}(x)}^2}{{ f^\prime(x)}^6} \\
%&= 1 - \frac{{f^\prime (x)}^2 - f(x)\, f^{\prime \prime}(x)}{f^\prime(x)^2} -\frac{{f(x)}^2\, f^{(3)}(x)\, f^\prime(x) - 3\, {f(x)}^2\, { f^{\prime \prime}(x)}^2 + 2\, f(x)\, { f^\prime(x)}^2\, f^{\prime \prime}(x)}{{ f^\prime(x)}^4} \\
%&= 1 - 1 - \frac{f(x)\, f^{\prime \prime}(x)}{f^\prime(x)^2}
%-\frac{{f(x)}^2\, f^{(3)}(x)\, f^\prime(x) - 3\, {f(x)}^2\, { f^{\prime \prime}(x)}^2 + 2\, f(x)\, { f^\prime(x)}^2\, f^{\prime \prime}(x)}{{ f^\prime(x)}^4} \\
&= \frac{3\, {f(x)}^2\, { f^{\prime \prime}(x)}^2}{2\, { f^\prime(x)}^4} - \frac{{f(x)}^2\, f^{(3)}(x)}{2\, { f^\prime(x)}^3} \\
\end{aligned}
\]

\[
\begin{aligned}
g^\prime (\alpha) &= \frac{3\, {f(\alpha)}^2\, { f^{\prime \prime}(\alpha)}^2}{2\, { f^\prime(\alpha)}^4} - \frac{{f(\alpha)}^2\, f^{(3)}(\alpha)}{2\, { f^\prime(\alpha)}^3} \\
&= \frac{3\, {(0)}^2\, { f^{\prime \prime}(\alpha)}^2}{2\, { f^\prime(\alpha)}^4} - \frac{{(0)}^2\, f^{(3)}(\alpha)}{2\, { f^\prime(\alpha)}^3} \\
&= \frac{0}{2\, { f^\prime(\alpha)}^4} - \frac{0}{2\, { f^\prime(\alpha)}^3} \\
&= 0
\end{aligned}
\]

Likewise when differentiating $g^\prime(x)$ we will have a function
that is $0$ when $x = \alpha$ since $f(\alpha) = 0$,

\[
\begin{aligned}
g^{\prime \prime} (x) &= \frac{3\, f(x)\, {f^{\prime \prime}(x)}^2}{{ f^\prime(x)}^3} -
\frac{6\, {f(x)}^2\, {f^{\prime \prime}(x)}^3}{{ f^\prime(x)}^5} -
\frac{{f(x)}^2\,  f^{(4)}(x)}{2\, { f^\prime(x)}^3} - \frac{f(x)\,
  f^{(3)}(x)}{{ f^\prime(x)}^2} + \frac{9\, {f(x)}^2\,  f^{(3)}(x)\,
   f^{\prime \prime}(x)}{2\, { f^\prime(x)}^4} \\
g^{\prime \prime} (\alpha) &= 0
\end{aligned}
\]

}
