\textbf{Polynomial Interpolation:}
Suppose you want to interpolate to the data
$(x_i, y_i)$, $i=0,\dots,n$ by a polynomial of degree $n$. Recall that
the interpolating polynomial $p$ can be written in its Lagrange form
as
\[
p(x) = \sum_{i=0}^n y_i L_i(x)\text{    where    } L_i(x) =
\frac{\prod_{i\ne j} (x - x_j)}{\prod_{i \ne j} (x_i - x_j)}.
\]
Show that
\[\sum_{i=0}^n x_i^j L_i(x) = x^j\text{    for    } j=0,\dots,n.\]

{\color{blue}
If $y_i = x_i^j$ then we have,

\[
\begin{aligned}
p(x) &= \sum_{i=0}^n x_i^j L_i(x) \\
&= \sum_{i=0}^n x_i^j \frac{\prod_{i\ne j} (x - x_j)}{\prod_{i \ne j}
  (x_i - x_j)} \\
&= \sum_{i=0}^n x_i^j
\frac{(x - x_0)(x - x_1)\cdots (x - x_{j-1})(x - x_{j+1}) \cdots (x - x_n)}
{(x_i - x_0)(x_i - x_1)\cdots (x_i - x_{j-1})(x_i - x_{j+1}) \cdots (x_i - x_n)} \\
&= \sum_{i=0}^n x_i^j
\frac{(x - x_0)(x - x_1)\cdots (x - x_{j-1})(x - x_{j+1}) \cdots (x - x_n)}
{(x_i - x_0)(x_i - x_1)\cdots (x_i - x_{j-1})(x_i - x_{j+1}) \cdots
  (x_i - x_n)}
\frac{(x_i - x_j)}{(x_i - x_j)} \\
&= \sum_{i=0}^n
\frac{(x_i^{j+1} - x_i^j x_j)(x - x_0)(x - x_1)\cdots (x - x_{j-1})(x - x_{j+1}) \cdots (x - x_n)}
{n (x_i - x_j)(x_i - x_0)(x_i - x_1)\cdots (x_i - x_{j-1})(x_i - x_{j+1}) \cdots
  (x_i - x_n)} \\
&= \sum_{i=0}^n
\frac{x^j (x_i - x_j)(x_i - x_0)(x_i - x_1)\cdots (x_i - x_{j-1})(x_i - x_{j+1}) \cdots
  (x - x_n)}
{n (x_i - x_j)(x_i - x_0)(x_i - x_1)\cdots (x_i - x_{j-1})(x_i - x_{j+1}) \cdots
  (x_i - x_n)} \\
&= x^j \sum_{i=0}^n
\frac{(x_i - x_j)(x_i - x_0)(x_i - x_1)\cdots (x_i - x_{j-1})(x_i - x_{j+1}) \cdots
  (x - x_n)}
{n (x_i - x_j)(x_i - x_0)(x_i - x_1)\cdots (x_i - x_{j-1})(x_i - x_{j+1}) \cdots
  (x_i - x_n)} \\
&= x^j \sum_{i=0}^n
\frac{1} {n} \\
&= x^j
\end{aligned}
\]


}
