\textbf{Uniqueness of the interpolating polynomial:} Assume you are
given the data
\[\begin{aligned}
x_i\;&: \,\, 1 \,\, 2 \,\, 4 \,\, 8 \\
y_i\;&: \,\, 1 \,\, 2 \,\, 3 \,\, 4
\end{aligned}\] Construct the interpolating polynomial using

\begin{enumerate}
\item the power form
\item the Lagrange form
\item the Newton form,
\end{enumerate}
and show that they all yield the same polynomial.

{\color{blue}

\begin{enumerate}
\item[(a) the power form]

\[
\begin{aligned}
  p(x) &= a_0 + a_1 x + a_2 x^2 + a_3 x^3 \\
  \Rightarrow p(x) &= V_n \vect{a} = \vect{y} \\
p(x) &=
\left(\begin{array}{cccc}
  1 & x_0 & x_0^2 & x_0^3 \\
  1 & x_1 & x_1^2 & x_1^3 \\
  1 & x_2 & x_2^2 & x_2^3 \\
  1 & x_3 & x_3^2 & x_3^3
\end{array}\right)
\left(\begin{array}{c}
  a_0 \\
  a_1 \\
  a_2 \\
  a_3
\end{array}\right)
= \left(\begin{array}{c}
  y_0 \\
  y_1 \\
  y_2 \\
  y_3
\end{array}\right) \\
p(x) &= \left(\begin{array}{cccc}
  1 & 1 & 1 & 1 \\
  1 & 2 & 4 & 8 \\
  1 & 4 & 16 & 64 \\
  1 & 8 & 64 & 512
\end{array}\right)
\left(\begin{array}{c}
  a_0 \\
  a_1 \\
  a_2 \\
  a_3
\end{array}\right)
= \left(\begin{array}{c}
  1 \\
  2 \\
  3 \\
  4
\end{array}\right) \\
p(x) &= \left(\begin{array}{cccc}
  1 & 1 & 1 & 1 \\
  1 & 2 & 4 & 8 \\
  1 & 4 & 16 & 64 \\
  1 & 8 & 64 & 512
\end{array}\right)
\left(\begin{array}{c}
  - \frac{10}{21}\\
  \frac{7}{4}\\
  - \frac{7}{24}\\
  \frac{1}{56}
\end{array}\right)
= \left(\begin{array}{c}
  1 \\
  2 \\
  3 \\
  4
\end{array}\right) \\
p(x) &= \frac{1}{56} x^3 - \frac{7}{24} x^2 + \frac{7}{4} x - \frac{10}{21}
\end{aligned}
\]

\item[(b) the Lagrange form]

\[
L(x) = \frac{\prod_{i \ne j} (x - x_j)}{\prod_{i \ne j} (x_i - x_j)}
\]

\[
\begin{aligned}
  p(x) &= \sum_{i=0}^n y_i L(x) \\
  p(x) &= 1 \frac{(x-2)(x-4)(x-8)}{(1-2)(1-4)(1-8)} + 2 \frac{(x-1)(x-4)(x-8)}{(2-1)(2-4)(2-8)} \\
  &    + 3 \frac{(x-1)(x-2)(x-8)}{(4-1)(4-2)(4-8)} + 4 \frac{(x-1)(x-2)(x-4)}{(8-1)(8-2)(8-4)}\\
  p(x) &= \frac{x^3 - 14\, x^2 + 56\, x - 64}{-21} + \frac{x^3 - 13\, x^2 + 44\, x - 32}{12} \\
&    + \frac{x^3 - 11\, x^2 + 26\, x - 16}{-24} + \frac{x^3 - 7\, x^2 + 14\, x - 8}{168} \\
p(x) &= \frac{1}{56} x^3 - \frac{7}{24} x^2 + \frac{7}{4} x - \frac{10}{21}
\end{aligned}
\]

\item[(c) the Newton form]

\[
\begin{aligned}
p_k(x) &= \sum_{i=0}^k c_i \prod_{j=0}^{i-1} (x - x_j) \\
\Rightarrow p_0(x) &= c_0 \\
p_1(x) &= p_0(x) + c_1(x -x_0) \\
p_2(x) &= p_1(x) + c_2(x -x_0)(x - x_1) \\
p_3(x) &= p_2(x) + c_3(x -x_0)(x - x_1)(x - x_2) \\
\Rightarrow p_0(x) &= y_0 \\
p_1(x) &= p_0(x) + \frac{y_1 - P_0(x_1)}{(x_1 - x_0)} (x -x_0) \\
p_2(x) &= p_1(x) + \frac{y_2 - P_1(x_2)}{(x_2 - x_0)(x_2 - x_1)} (x -x_0)(x - x_1) \\
p_3(x) &= p_2(x) + \frac{y_3 - P_2(x_3)}{(x_3 - x_0)(x_3 - x_1)(x_3 - x_2)} (x -x_0)(x - x_1)(x - x_2) \\
\Rightarrow p_0(x) &= 1 \\
p_1(x) &= p_0(x) + \frac{2 - P_0(2)}{(2 - 1)} (x -1) \\
p_2(x) &= p_1(x) + \frac{3 - P_1(4)}{(4 - 1)(4 - 2)} (x -1)(x - 2) \\
p_3(x) &= p_2(x) + \frac{4 - P_2(8)}{(8 - 1)(8 - 2)(8 - 4)} (x -1)(x - 2)(x - 4) \\
\end{aligned}
\]
\[
\begin{aligned}
\Rightarrow p_0(x) &= 1 \\
p_1(x) &= 1 + \frac{2 - 1}{(2 - 1)} (x -1) \\
&= 1 + \frac{1}{1} (x - 1) \\
&= x \\
p_2(x) &= x + \frac{3 - 4}{(4 - 1)(4 - 2)} (x -1)(x - 2) \\
&= x - \frac{1}{6} (x - 1) (x - 2) \\
&= x - \frac{x^2 - 3x + 2}{6} \\
&= - \frac{x^2}{6} + \frac{3\, x}{2} - \frac{1}{3} \\
p_3(x) &= - \frac{x^2}{6} + \frac{3\, x}{2} - \frac{1}{3} + \frac{4 - 1}{(8 - 1)(8 - 2)(8 - 4)} (x -1)(x - 2)(x - 4) \\
&= - \frac{x^2}{6} + \frac{3\, x}{2} - \frac{1}{3} + \frac{3}{168} (x -1)(x-2)(x-4) \\
&= - \frac{x^2}{6} + \frac{3\, x}{2} - \frac{1}{3} + \frac{3}{168} \left(x^3 - 7\, x^2 + 14\, x - 8\right) \\
&= - \frac{x^2}{6} + \frac{3\, x}{2} - \frac{1}{3} + \frac{3\, x^3 - 21\, x^2 + 42\, x - 24}{168} \\
&= \frac{1}{56} x^3 - \frac{7}{24} x^2 + \frac{7}{4} x - \frac{10}{21} \\
\Rightarrow P(x) &= \frac{1}{56} x^3 - \frac{7}{24} x^2 + \frac{7}{4} x - \frac{10}{21}
\end{aligned}
\]

\end{enumerate}

}
