\textbf{Example for Gram Schmidt Process.} Use the Gram-Schmidt
Process to find a basis of \[\mathrm{span}\{1, x, e^x\}\] that is orthonormal
with respect to the inner product \[(f,g) = \int_0^1 f(x) g(x)
\mathrm{d}x.\]

{\color{blue}


\[
b = \text{span} \{ 1, x, e^x \}
\]

\[
\begin{aligned}
z_k &= b_k - \sum_{i=0}^{k-1} (b_k, q_i) q_i \\
q_k &= \frac{z_k}{||z_k||}
\end{aligned}
\]

\[
\begin{aligned}
z_0 &= 1 \\
q_0 &= \frac{b_0}{|| b_0 ||} = \frac{1}{|| 1 ||} = 1 \\
\end{aligned}
\]

\[
\begin{aligned}
z_1 &= x - \int_0^1 t \text{d}t \\
&= x - \frac{1}{2} \\
q_1 &= \frac{x - \frac{1}{2}}{(\int_0^1 (t - \frac{1}{2})^2 \text{d}t)^{\frac{1}{2}}} \\
&= \frac{x - \frac{1}{2}}
{(\int_0^1 t^2 - t + \frac{1}{4} \text{d}t)^{\frac{1}{2}}} \\
&= \frac{x - \frac{1}{2}}
{(\frac{1}{12})^{\frac{1}{2}}} \\
&= \frac{x - \frac{1}{2}}
{\frac{1}{2 \sqrt{3}}} \\
&= \sqrt{3}(2x - 1)
\end{aligned}
\]

\[
\begin{aligned}
z_2 &= e^x - \int_0^1 e^t \text{d}t - \int_0^1 e^t \sqrt{3} (2t - 1)
\text{d}t (\sqrt{3} (2x-1)) \\
&= e^x - (e - 1) - \sqrt{3} \int_0^1 e^t 2 t - e^t \text{d}t (\sqrt{3}
(2x-1)) \\
&= e^x - e + 1 - (6x - 3) (2 \int_0^1 e^t t \text{d}t - (e-1)) \\
&= e^x - e + 1 - (6x - 3) (2 (e^t t \bigg|_0^1 - \int_0^1 e^t
\text{d}t) - (e-1)) \\
&= e^x - e + 1 - (6x - 3) (2 e - 2 (e-1) - (e-1)) \\
&= e^x - e + 1 - (6x - 3) (2e - 2e + 2 - e + 1) \\
&= e^x - e + 1 - (6x - 3) (3 - e) \\
&= e^x - e + 1 - (18x - 6ex - 9 + 3e) \\
&= e^x - e + 1 - 18x + 6ex + 9 - 3e \\
&= e^x - 4e - 18x + 6ex + 10 \\
q_2 &= \frac{
e^x - 4e - 18x + 6ex + 10
}{
|| e^x - 4e - 18x + 6ex + 10 ||
}\\
q_2 &= \frac{
e^x - 4e - 18x + 6ex + 10
}{
(\int_0^1  (e^x - 4e - 18x + 6ex + 10)^2 \text{d}t)^{\frac{1}{2}}
}\\
q_2 &= \frac{
e^x - 4e - 18x + 6ex + 10
}{
(\int_0^1
  e^{2x} - 4 e^x e - 18 e^x x + 6 e^x e x + 10 e^x
- 4 e^x e + 16 e^2 + 72 e x - 24 e^2 x - 40 e
- 18 e^x x + 72 e x + 324 x^2 - 108 e x^2 - 180 x
+ 6 e^x e x - 24 e^2 x - 108 e x^2 + 36 e^2 x^2 + 60 e x
+ 10 e^x - 40 e - 180x + 60e x + 100
\text{d}t)^{\frac{1}{2}}
}\\
q_2 &= \frac{
e^x - 4e - 18x + 6ex + 10
}{
(\int_0^1
e^{2x} - 360 x - 80 e + 16 e^2 + 20 e^x
+ 264 x e - 48 x e^2 - 216 x^2 e + 36 x^2 e^2
- 8 e e^x - 36 x e^x + 324 x^2 + 12 x e e^x
+ 100
\text{d}t)^{\frac{1}{2}}
}\\
q_2 &= \frac{
e^x - 4e - 18x + 6ex + 10
}{
\sqrt{
  20 e - \frac{7 e^2}{2} - \frac{57}{2}
}
}\\
\end{aligned}
\]



}
