\textbf{The Three Term Recurrence Relation} Let the inner product
$(f,g)$ be defined by \[(f,g) = \int_a^b w(x) f(x) g(x) \mathrm{d}x\]
(where $w$ is a positive weight function). Prove that the sequence of
polynomials defined by
\[
\begin{aligned}
Q_n &= (x - a_n) Q_{n-1} - b_n Q_{n-2} \\
Q_0 &= 1 \\
Q_1 &= x - a_n \\
a_n &= \frac{(x Q_{n-1}, Q_{n-1})}{(Q_{n-1}, Q_{n-1})} \\
b_n &= \frac{(x Q_{n-1}, Q_{n-2})}{(Q_{n-2}, Q_{n-2})}
\end{aligned}
\]
is orthogonal with respect to (3). Note that the proof of this fact
uses the property \[(xf, g) = (f, xg)\] of (3).

{\color{blue}

Proof by induction
\[
\begin{aligned}
(Q_0, Q_1) &= (1, x - \frac{(x, 1)}{(1,1)}) \\
           &= (1,x) - (1, \frac{(x,1)}{(1,1)}) \\
           &= (1,x) - (1,1) \frac{(x,1)}{(1,1)} \\
           &= (1,x) - (1,x) = 0.
\end{aligned}
\]

Assume that $Q_0, Q_1, \dots, Q_{n-1}$ are all orthogonal to each
other, and that $k<n$. Then,

\[
\begin{aligned}
(Q_n, Q_k) &= \left( \left( x - \frac{(x Q_{n-1}, Q_{n-1})}{(Q_{n-1},
Q_{n-1})} \right) Q_{n-1} - \frac{(x Q_{n-1}, Q_{n-2})}{(Q_{n-2},
Q_{n-2})} Q_{n-2}, Q_k \right) \\
&= (x Q_{n-1}, Q_k) - \frac{(x Q_{n-1}, Q_{n-1})}{(Q_{n-1}, Q_{n-1})}
(Q_{n-1}, Q_k) - \frac{(x Q_{n-1}, Q_{n-2})}{(Q_{n-2}, Q_{n-2})}
(Q_{n-2}, Q_k)
\end{aligned}
\]

Here we have three cases: $k = n-1$, $k = n-2$, $k < n-2$. Checking
each of these,

\[
\begin{aligned}
k = n-1: &= (x Q_{n-1}, Q_{n-1}) - (x Q_{n-1}, Q_{n-1}) = 0 \\
k = n-2: &= (x Q_{n-1}, Q_{n-2}) - (x Q_{n-1}, Q_{n-2}) = 0 \\
k < n-2: &= (x Q_{n-1}, Q_k) \\
&= (Q_{n-1}, x Q_k) \\
&= \left(Q_{n-1}, \sum_{i=0}^{n-2} \alpha_i Q_i\right)
= \sum_{i=0}^{n-2} \alpha_i (Q_{n-1}, Q_i) = 0
\end{aligned}
\]

% TODO explain the steps clearly so that it's not just a direct copy
% of the notes

}
