\textbf{Recurrence Relation.} Consider the inner product \[(f,g) =
\int_{-1}^1 f(x) g(x) \mathrm{d}x.\] Use the recurrence relation (4)
to compute $Q_i$ for $i=0,1,2,3,4,5$.


{\color{blue}

\[
\begin{aligned}
Q_0 &= 1 \\
\end{aligned}
\]

\[
\begin{aligned}
a_1 &= \frac{(x Q_0, Q_0)}{(Q_0, Q_0)} = \frac{(x,1)}{(1,1)} \\
Q_1 &= x - \frac{(x,1)}{(1,1)}  \\
    &= x \\
\end{aligned}
\]

For the interval $[-1, 1]$ the dot production of any odd and even
polynomial will result in the integral of an odd function which will
be zero, thus $a_i = 0$,

\[
\begin{aligned}
a_2 &= \frac{(x Q_1, Q_1)}{(Q_1, Q_1)}\\
    &= \frac{(x,1)}{(1,1)} \\
    &= \frac{(x^2, x)}{(x,x)} \\
    &= 0
b_2 &=  \frac{(x Q_1, Q_0)}{(Q_0, Q_0)} \\
    &=  \frac{(x^2, 1)}{(1,1)} \\
    &=  \frac{2}{3} \\
Q_2 &= (x-a_2) Q_1 - b_2 Q_0 \\
&= (x - a_2) x - b_2 (1) \\
&= x^2 - \frac{2}{3} \\
\end{aligned}
\]

\[
\begin{aligned}
a_3 &= \frac{(x Q_2, Q_2)} {(Q_2, Q_2)}\\
    &= \frac{(x^3 - \frac{2}{3} x, x^2 - \frac{2}{3})}{(x^2 - \frac{2}{3}, x^2 - \frac{2}{3})} \\
    &= \frac{\int_{-1}^1 (x^3 - \frac{2}{3} x) (x^2 - \frac{2}{3}) \textrm{d}x}{\int_{-1}^1 (x^2 - \frac{2}{3})^2 \textrm{d}x}\\
    &= \frac{0}{2/5} \\
    &= 0 \\
b_3 &= \frac{(x Q_2, Q_1)}{(Q_1, Q_1)}\\
    &= \frac{(x^3 - \frac{2}{3}x, x)}{(x,x)}\\
    &= \frac{-2/45}{2/3} \\
    &= -\frac{1}{15} \\
Q_3 &= x(x^2 - \frac{2}{3}) + \frac{1}{15} x \\
    &= x^3 - \frac{2}{3} x + \frac{1}{15} x \\
    &= x^3 - \frac{3}{5} x
\end{aligned}
\]

\[
\begin{aligned}
a_4 &= \frac{(x Q_3, Q_3)}{(Q_3, Q_3)}\\
    &= \frac{\int_{-1}^1 x (x^3 - \frac{3}{5} x)^2 \textrm{d}x}{
    \int_{-1}^1 (x^3 - \frac{3}{5} x)^2 \textrm{d}x} \\
    &= \frac{0}{8/175} \\
    &= 0 \\
b_4 &= \frac{(x Q_3, Q_2)}{(Q_2, Q_2)} \\
    &= \frac{\int_{-1}^1 x (x^3 - \frac{3}{5} x) (x^2 - \frac{2}{3}) \textrm{d}x}{\int_{-1}^1 (x^2 - \frac{2}{3})^2 \textrm{d}x} \\
    &= \frac{8/175}{2/5} \\
    &= \frac{4}{35} \\
Q_4 &= (x- a_4) Q_3 - b_4 Q_2 \\
    &= x (x^3 - \frac{3}{5} x) - \frac{4}{35} (x^2 - \frac{2}{3}) \\
    &= x^4 - \frac{3}{5} x^2 - \frac{4}{35} x^2 - \frac{2}{3}
    (\frac{4}{35}) \\
    &= x^4 - \frac{5}{7} x^2 - \frac{8}{105}
\end{aligned}
\]

\[
\begin{aligned}
a_5 &= \frac{(x Q_4, Q_4)}{(Q_4, Q_4)}\\
    &= \frac{\int_{-1}^1 x (x^4 - \frac{5}{7} x^2
    - \frac{8}{105})^2 \textrm{d}x}{\int_{-1}^1 (x^4 - \frac{5}{ 7}
    x^2 - \frac{8}{105})^2 \textrm{d}x}  \\
    &= \frac{0}{152/3675} \\
b_5 &= \frac{(x Q_4, Q_3)}{(Q_3, Q_3)} \\
    &= \frac{\int_{-1}^1 x (x^4 - \frac{5}{7} x^2 - \frac{8}{105})(x^3
    - \frac{3}{5} x) \textrm{d}x}{\int_{-1}^1 (x^3 - \frac{3}{5}
    x)^2 \textrm{d}x}\\
    &= \frac{8/441}{8/175} \\
    &= \frac{25}{63} \\
Q_5 &= (x - a_5) Q_4 - b_5 Q_3 \\
    &= x (x^4 - \frac{5}{7} x^2 - \frac{8}{105}) - \frac{25}{63} (x^3
    - \frac{3}{5} x) \\
    &= x^5 - \frac{5}{7} x^3 - \frac{8}{105} x - \frac{25}{63} x^3
    - \frac{3}{5} (\frac{25}{63}) x \\
    &= x^5 - \frac{10}{9} x^3 - \frac{11}{35} x
\end{aligned}
\]

}
