\textbf{More on the Recurrence Relation.} Remember that a key property
of the inner products for which we established the three term relation
was that $(xf,g) = (f,xg)$. Find an inner product that violates that
rule, and for which the recurrence relation does indeed fail to yield
orthogonal polynomials. (Thus use the recurrence relation to construct
the first few polynomials, until you find two that are not orthogonal.)

{\color{blue}
Let the inner product $(f,g)$ be defined as
\[
(f,g) = \int_{-1}^1 f(x)g(x) + f^\prime(x) g^\prime(x) \textrm{d}x
\]
Then the following properties hold
\begin{align*}
(f,g) &= \int_{-1}^1 f(x)g(x) + f^\prime(x) g^\prime(x) \textrm{d}x\\
      &= \int_{-1}^1 g(x)f(x) + g^\prime(x) f^\prime(x) \textrm{d}x\\
      &= (g,f)\\
(f+g, h) &= \int_{-1}^1 (f(x) + g(x))h(x) + (f(x) + g(x))^\prime h^\prime(x) \textrm{d}x\\
         &= \int_{-1}^1 f(x)h(x) + g(x)h(x) + (f^\prime(x) + g^\prime(x)) h^\prime(x) \textrm{d}x\\
         &= \int_{-1}^1 f(x)h(x) + g(x)h(x) + f^\prime(x) h^\prime(x) + g^\prime(x) h^\prime(x) \textrm{d}x\\
         &= \int_{-1}^1 f(x)h(x) + f^\prime(x) h^\prime(x) + g(x)h(x) + g^\prime(x) h^\prime(x) \textrm{d}x\\
         &= \int_{-1}^1 f(x)h(x) + f^\prime(x) h^\prime(x) \textrm{d}x
         + \int_{-1}^1 g(x)h(x) + g^\prime(x) h^\prime(x) \textrm{d}x\\
         &= (f,h) + (g,h) \\
(f,f) &= \int_{-1}^1 f(x)f(x) + f^\prime(x) f^\prime(x) \textrm{d}x\\
      &\ge 0 \\
\end{align*}
However the property which our recurrence relation relies on $(xf,g) =
(f, xg)$ does not,
\begin{align*}
(xf,g) &= \int_{-1}^1 xf(x)g(x) + (xf(x))^\prime g^\prime(x) \textrm{d}x\\
(f,xg) &= \int_{-1}^1 xf(x)g(x) + f^\prime(x) (xg(x))^\prime \textrm{d}x\\
(xf(x))^\prime &\ne (xg(x))^\prime\\
\Rightarrow (xf,g) &\ne (f,xg)
\end{align*}

If we test out our recurrence relation we find the following
polynomials,

\begin{align*}
Q_0 &= 1 \\
Q_1 &= x \\
a_2 &= \frac{(xQ_1,Q_1)}{(Q_1, Q_1)} = 0 \\
b_2 &= \frac{(xQ_1,Q_0)}{(Q_0, Q_0)} = \frac{1}{3} \\
Q_2 &= x^2 - \frac{1}{3} \\
a_3 &= \frac{(xQ_2,Q_2)}{(Q_2, Q_2)} = 0 \\
b_3 &= \frac{(xQ_2,Q_1)}{(Q_1, Q_1)} = \frac{17}{30} \\
Q_3 &= x^3 - \frac{9}{10} \\
a_4 &= \frac{(xQ_3,Q_3)}{(Q_3, Q_3)} = 0 \\
b_4 &= \frac{(xQ_3,Q_2)}{(Q_2, Q_2)} = \frac{39}{140} \\
Q_4 &= x^4 - \frac{33}{28} x^2 + \frac{13}{140} \\
\end{align*}

Checking the orthogonality of these polynomials we find that our
fourth polynomial is no longer orthogonal to our first, and we can see
that our recurrence relation has failed to find orthogonal polynomials.
\begin{align*}
(Q_0, Q_1) &= 0 \\
(Q_2, Q_0) &= 0 \\
(Q_2, Q_1) &= 0 \\
(Q_3, Q_0) &= 0 \\
(Q_3, Q_1) &= 0 \\
(Q_3, Q_2) &= 0 \\
(Q_4, Q_0) &\boxed{= -\frac{1}{5} \ne 0} \\
\end{align*}


}
